proof/DependentTypeLemmas.v
@@ -37,7 +37,7 @@
 Require Import Model.ADT  Model.Hardware Model.MAL Arith Model.Lib StateLib.
 Require Import Coq.Logic.ProofIrrelevance Omega.
 
-
+(** ADT : level **)
 Lemma levelEqBEqNatTrue :
 forall l l' : level, StateLib.Level.eqb l l' = true -> l = l' .
  Proof.
@@ -108,6 +108,60 @@ simpl; omega.
 now contradict H.
 Qed.
 
+Lemma levelPredMinus1: forall l l' , StateLib.Level.eqb l fstLevel = false -> StateLib.Level.pred l = Some l' -> l' = CLevel (l - 1).
+Proof.
+intros. 
+unfold StateLib.Level.pred  in *.
+assert (l > 0).
+{ apply levelEqBEqNatFalse0.
+  assumption. }
+case_eq (gt_dec l 0).
+* intros.
+  rewrite H2 in H0.
+  inversion H0.
+  unfold CLevel.
+  case_eq (lt_dec (l - 1) nbLevel).
+  intros. subst.   
+  assert (ADT.CLevel_obligation_1 (l - 1) l0  = StateLib.Level.pred_obligation_1 l g ).
+  apply proof_irrelevance. 
+  rewrite H4. reflexivity.
+  intros.
+  destruct l.
+  subst. 
+  simpl in *.
+  contradict H3.
+  omega.
+* intros.
+  contradict H1.
+  assumption.
+Qed.
+
+Lemma levelEqNat : 
+forall a b , a < nbLevel -> b < nbLevel -> CLevel a = CLevel b -> a = b.
+Proof.
+intros a b Ha Hb Hab.
+ unfold CLevel in *.
+ case_eq (lt_dec a nbLevel );intros g Ha'.
+ + rewrite Ha' in Hab.
+   case_eq (lt_dec b nbLevel);intros p Hb'.
+   - rewrite Hb' in Hab.
+     inversion Hab. intuition.
+   - omega.
+ + omega.  
+Qed.
+
+Lemma level_gt : 
+forall x x0, x - x0 < nbLevel ->  CLevel (x - x0) > 0 -> x > x0.
+Proof.
+intros.
+unfold CLevel in *.
+case_eq (lt_dec (x - x0) nbLevel ).
+intros. rewrite H1 in H0.
+simpl in *. omega.
+intros. contradict H1. omega.       
+Qed.   
+
+(**** ADT : page **)
 Lemma isDefaultPageFalse : forall p,   (defaultPage =? pa p) = false -> pa p <> defaultPage .
 Proof.
 intros. 
@@ -163,48 +217,8 @@ subst.
 intuition.
 Qed.
 
-Lemma levelPredMinus1: forall l l' , StateLib.Level.eqb l fstLevel = false -> StateLib.Level.pred l = Some l' -> l' = CLevel (l - 1).
-Proof.
-intros. 
-unfold StateLib.Level.pred  in *.
-assert (l > 0).
-{ apply levelEqBEqNatFalse0.
-  assumption. }
-case_eq (gt_dec l 0).
-* intros.
-  rewrite H2 in H0.
-  inversion H0.
-  unfold CLevel.
-  case_eq (lt_dec (l - 1) nbLevel).
-  intros. subst.   
-  assert (ADT.CLevel_obligation_1 (l - 1) l0  = StateLib.Level.pred_obligation_1 l g ).
-  apply proof_irrelevance. 
-  rewrite H4. reflexivity.
-  intros.
-  destruct l.
-  subst. 
-  simpl in *.
-  contradict H3.
-  omega.
-* intros.
-  contradict H1.
-  assumption.
-Qed.
 
-Lemma levelEqNat : 
-forall a b , a < nbLevel -> b < nbLevel -> CLevel a = CLevel b -> a = b.
-Proof.
-intros a b Ha Hb Hab.
- unfold CLevel in *.
- case_eq (lt_dec a nbLevel );intros g Ha'.
- + rewrite Ha' in Hab.
-   case_eq (lt_dec b nbLevel);intros p Hb'.
-   - rewrite Hb' in Hab.
-     inversion Hab. intuition.
-   - omega.
- + omega.  
-Qed.
-
+(** ADT : index **)
 Lemma indexEqFalse : 
 forall a b : nat , a < tableSize -> b < tableSize -> a <> b -> CIndex a <> CIndex b.
 Proof.
@@ -223,7 +237,7 @@ case_eq (lt_dec a tableSize).
 + intros. contradict H. intuition.
 Qed. 
 
-Lemma ltbIndexTrue : 
+Lemma indexltbTrue : 
 forall i1 i2 : index , 
 StateLib.Index.ltb i1 i2 = true -> i1 < i2.
 Proof. intros. unfold MALInternal.Index.ltb in H. 
@@ -231,7 +245,7 @@ apply NPeano.Nat.ltb_lt in H.
 assumption.
 Qed. 
 
-Lemma ltbIndexFalse : 
+Lemma indexltbFalse : 
 forall i1 i2 : index , 
 StateLib.Index.ltb i1 i2 = false -> i1 >= i2.
 Proof.
@@ -241,17 +255,6 @@ apply not_lt.
 apply NPeano.Nat.ltb_nlt in H.
 omega.  
 Qed. 
-
-Lemma level_gt : 
-forall x x0, x - x0 < nbLevel ->  CLevel (x - x0) > 0 -> x > x0.
-Proof.
-intros.
-unfold CLevel in *.
-case_eq (lt_dec (x - x0) nbLevel ).
-intros. rewrite H1 in H0.
-simpl in *. omega.
-intros. contradict H1. omega.       
-Qed.   
 
 Lemma indexBoundEq : 
 forall i : index , i>= CIndex (tableSize - 1) -> i =  CIndex (tableSize - 1). 
@@ -276,15 +279,357 @@ unfold  tableSizeLowerBound in * . omega. omega.
 Qed.
 
 Lemma indexDiffLtb :
-forall i1 i2 : index, i2 < i1 \/ i1 < i2 -> i2 <> i1.
+forall i1 i2 : index, i2 < i1 \/ i1 < i2 <-> i2 <> i1.
 Proof.
 intros.
-destruct i1, i2.
-simpl in *. unfold not.
+split;destruct i1, i2;
+simpl in *.
+ unfold not;
+intros;
+inversion H0; omega.
 intros.
-inversion H0. omega.
+apply nat_total_order.
+unfold not in *; intros; subst.
+apply H; f_equal.
+apply proof_irrelevance.
 Qed.
 
+Lemma indexEqId : 
+forall i : index, CIndex i = i. 
+Proof.
+intros.
+unfold CIndex.
+destruct i.
+simpl.
+case_eq(lt_dec i tableSize); intros.
+assert(ADT.CIndex_obligation_1 i l = Hi) by apply proof_irrelevance.
+subst. reflexivity.
+now contradict Hi.
+Qed.
+
+Lemma indexMaxEqFalseLt : 
+forall idx : index, idx <> CIndex (tableSize - 1) -> idx < tableSize - 1.
+Proof.
+intros.
+unfold CIndex in *.
+case_eq (lt_dec (tableSize - 1) tableSize).
+intros .
+rewrite H0 in *.
+destruct idx.
+simpl in *.
+apply not_ge.
+unfold not.
+intros.
+contradict H.
+assert (i = tableSize - 1).
+omega.
+subst.
+f_equal.
+apply proof_irrelevance.
+intros.
+assert(tableSizeLowerBound < tableSize) by apply tableSizeBigEnough.
+omega.
+Qed.
+
+Lemma indexMaxEqFalseLt1 : 
+forall idx : index, idx <> CIndex (tableSize - 1) -> idx < CIndex (tableSize - 1).
+Proof.
+intros.
+unfold CIndex in *.
+case_eq (lt_dec (tableSize - 1) tableSize).
+intros .
+rewrite H0 in *.
+destruct idx.
+simpl in *.
+apply not_ge.
+unfold not.
+intros.
+contradict H.
+assert (i = tableSize - 1).
+omega.
+subst.
+f_equal.
+apply proof_irrelevance.
+intros.
+assert(tableSizeLowerBound < tableSize) by apply tableSizeBigEnough.
+omega.
+Qed.
+
+Lemma noteqIndex a b:
+a < tableSizeLowerBound -> b < tableSizeLowerBound -> a<>b ->  
+CIndex a <> CIndex b.
+Proof.
+intros. 
+apply indexEqFalse;
+assert (tableSize > tableSizeLowerBound).
+apply tableSizeBigEnough.
+unfold tableSizeLowerBound in *.
+omega.  apply tableSizeBigEnough.
+unfold tableSizeLowerBound in *.
+omega. apply tableSizeBigEnough. omega.
+Qed.
+
+Lemma indexEqbTrue : 
+forall idx1 idx2 : index, true = StateLib.Index.eqb idx1 idx2 -> 
+idx1 = idx2.
+Proof.
+unfold StateLib.Index.eqb in *.
+intros.
+symmetry in H.
+apply beq_nat_true in H.
+destruct idx1; destruct idx2.
+simpl in *.
+subst.
+f_equal.
+apply proof_irrelevance.
+Qed.
+
+Lemma indexLtZero : 
+forall idx : index, idx < CIndex 0 -> False.
+Proof.
+intros.
+unfold CIndex in *.
+case_eq (lt_dec 0 tableSize); intros; rewrite H0 in *.
+destruct idx. simpl in *.
+omega.
+assert (tableSizeLowerBound < tableSize) by apply tableSizeBigEnough.
+omega.
+Qed.
+
+Lemma indexSEqbZeroOdd : 
+forall curidx idxsucc, 
+true = StateLib.Index.eqb curidx (CIndex 0) -> 
+StateLib.Index.succ curidx = Some idxsucc -> 
+Nat.Odd idxsucc.
+Proof.
+intros.
+apply indexEqbTrue in H.
+subst.
+unfold Index.succ in *.
+case_eq (lt_dec (CIndex 0 + 1) tableSize); intros; rewrite H in *.
+inversion H0.
+destruct idxsucc.
+inversion H2.
+subst.
+unfold Nat.Odd.
+eexists 0.
+simpl.
+unfold CIndex.
+case_eq (lt_dec 0 tableSize); intros.
+simpl. trivial.
+assert (tableSizeLowerBound < tableSize) by apply tableSizeBigEnough.
+omega.
+now contradict H0.
+Qed.
+
+Lemma indexZeroNotOdd : 
+forall idx idxsucc : index,
+idx < idxsucc -> 
+StateLib.Index.succ (CIndex 0) = Some idxsucc ->
+~ Nat.Odd idx.
+Proof.
+intros.
+unfold Index.succ in *.
+case_eq (lt_dec (CIndex 0 + 1) tableSize); intros; rewrite H1 in *.
+inversion H0.
+destruct idxsucc.
+inversion H3.
+subst.
+clear H0 H3.
+simpl in *.
+unfold CIndex in H.
+case_eq (lt_dec 0 tableSize); intros.
+simpl. rewrite H0 in *.
+simpl in *.
+unfold not.
+intros.
+unfold Nat.Odd in *.
+destruct H2.
+rewrite H2 in *.
+omega.
+assert (tableSizeLowerBound < tableSize) by apply tableSizeBigEnough.
+omega.
+now contradict H0.
+Qed.
+ 
+ Lemma indexSEqbZeroLt : 
+forall  idxsucc idx : index, 
+StateLib.Index.succ (CIndex 0)  = Some idxsucc -> 
+idx < idxsucc -> 
+idx = CIndex 0.
+Proof.
+intros.
+unfold Index.succ in *.
+case_eq (lt_dec (CIndex 0 + 1) tableSize); intros; rewrite H1 in *.
+inversion H.
+destruct idxsucc.
+inversion H3.
+subst.
+clear H H3 H1  l.
+simpl in *.
+unfold CIndex in *.
+case_eq (lt_dec 0 tableSize); intros; rewrite H in *.
+simpl in *.
+destruct idx.
+simpl in *.
+destruct i.
+f_equal.
+apply proof_irrelevance.
+omega.
+assert (tableSizeLowerBound < tableSize) by apply tableSizeBigEnough.
+omega.
+now contradict H0.
+Qed.
+
+Lemma indexSuccGt : 
+forall idx curidx iIndex : index,
+StateLib.Index.succ curidx = Some iIndex -> 
+idx < curidx -> 
+idx <> iIndex.
+Proof.
+intros.
+unfold Index.succ in *.
+case_eq (lt_dec(curidx + 1) tableSize); intros; rewrite H1 in *.
+simpl in *.
+destruct idx.
+simpl in *.
+destruct iIndex.
+inversion H.
+unfold not; intros.
+inversion H2.
+subst.
+omega.
+now contradict H.
+Qed.
+
+Lemma indexSuccEqFalse: 
+forall  curidx iIndex : index,
+StateLib.Index.succ curidx = Some iIndex -> 
+ curidx <> iIndex.
+Proof.
+intros.
+unfold Index.succ in *.
+case_eq (lt_dec(curidx + 1) tableSize); intros; rewrite H0 in *.
+simpl in *.
+destruct iIndex.
+inversion H.
+subst.
+clear H.
+unfold not; intros.
+destruct curidx.
+simpl in *.
+inversion H.
+omega.
+now contradict H.
+Qed.
+
+Lemma indexSuccSuccOddOr (curidx iIndex nextidx idx : index): 
+StateLib.Index.succ curidx = Some iIndex ->
+StateLib.Index.succ iIndex = Some nextidx -> 
+Nat.Odd curidx -> 
+Nat.Odd idx -> 
+idx < nextidx -> 
+idx = curidx \/ idx < curidx.
+Proof.
+intros.
+unfold StateLib.Index.succ in *.
+      destruct (lt_dec (curidx + 1) tableSize); try now contradict H.
+      inversion H; clear H.
+      destruct (lt_dec (iIndex + 1) tableSize); try now contradict H0.
+      inversion H0; clear H0.
+      destruct nextidx.
+      inversion H4; clear H4.
+      destruct iIndex.
+      simpl in *.
+      subst.
+      inversion H5; clear H5.
+      destruct curidx.
+      simpl in *.
+      destruct idx.
+      simpl in *.
+      rewrite <- H0 in H3.
+      clear H0 Hi l0 l Hi0 .
+      assert (i1 = i \/ i1 < i).
+      unfold Nat.Odd in *.
+      destruct H1 ; destruct H2.
+      
+      omega.
+      destruct H.
+      left.
+      subst.
+      f_equal.
+      apply proof_irrelevance.
+      right; trivial.
+Qed.
+      
+Lemma indexSuccSuccEvenOr (curidx iIndex nextidx idx : index): 
+StateLib.Index.succ curidx = Some iIndex ->
+StateLib.Index.succ iIndex = Some nextidx -> 
+Nat.Even curidx -> 
+Nat.Even idx -> 
+idx < nextidx -> 
+idx = curidx \/ idx < curidx.
+Proof.
+intros.
+unfold StateLib.Index.succ in *.
+      destruct (lt_dec (curidx + 1) tableSize); try now contradict H.
+      inversion H; clear H.
+      destruct (lt_dec (iIndex + 1) tableSize); try now contradict H0.
+      inversion H0; clear H0.
+      destruct nextidx.
+      inversion H4; clear H4.
+      destruct iIndex.
+      simpl in *.
+      subst.
+      inversion H5; clear H5.
+      destruct curidx.
+      simpl in *.
+      destruct idx.
+      simpl in *.
+      rewrite <- H0 in H3.
+      clear H0 Hi l0 l Hi0 .
+      assert (i1 = i \/ i1 < i).
+      destruct H1 ; destruct H2.
+      omega.
+      destruct H.
+      left.
+      subst.
+      f_equal.
+      apply proof_irrelevance.
+      right; trivial.
+Qed.
+
+Lemma indexSuccSuccEvenOddLt (curidx iIndex nextidx idx : index): 
+StateLib.Index.succ curidx = Some iIndex ->
+StateLib.Index.succ iIndex = Some nextidx -> 
+Nat.Even idx -> 
+Nat.Odd curidx -> 
+idx < nextidx -> 
+idx < iIndex -> 
+idx < curidx.
+Proof.
+intros.
+unfold StateLib.Index.succ in *.
+      destruct (lt_dec (curidx + 1) tableSize); try now contradict H.
+      inversion H; clear H.
+      destruct (lt_dec (iIndex + 1) tableSize); try now contradict H0.
+      inversion H0; clear H0.
+      destruct nextidx.
+      inversion H5; clear H5.
+      destruct iIndex.
+      simpl in *.
+      subst.
+      inversion H6; clear H6.
+      destruct curidx.
+      simpl in *.
+      destruct idx.
+      simpl in *.
+      destruct H1; destruct H2.
+      subst.
+      
+      omega.
+Qed.
+(** ADT : vaddr **)
 Lemma lengthVAddrNotZero (va : vaddr) : fstLevel < (length va -1).
 Proof. 
  unfold fstLevel.  destruct va.
@@ -293,6 +638,81 @@ Proof.
  intros. destruct level_d. simpl. omega. 
  Qed.
 
+Lemma CLevelMinusEq0 : 
+forall (a : level) b , CLevel (a -  b) = CLevel 0 ->   a = CLevel b \/ a < b. 
+Proof.
+intros.
+unfold CLevel in *.  
+case_eq (lt_dec (a - b) nbLevel );
+intros lab Hab; rewrite Hab in *.
+case_eq(lt_dec 0 nbLevel);
+intros l0 H0;
+rewrite H0 in*.
+inversion H.
+case_eq (lt_dec b nbLevel);
+intros lb Hb.
+simpl in *.
+apply NPeano.Nat.sub_0_le in H2.
+apply le_lt_or_eq in H2.
+destruct H2. 
+right; assumption.
+left.
+destruct a.
+simpl in *.
+subst.
+assert (Hl =  ADT.CLevel_obligation_1 b lb ) by 
+apply proof_irrelevance.
+subst. reflexivity.
+right; destruct a; simpl in *; omega.
+assert (0 < nbLevel) by apply nbLevelNotZero.
+now contradict H1.
+destruct a. simpl in *.
+omega.
+Qed.
+
+Lemma getNbLevelLe : 
+forall nbL, 
+Some nbL = StateLib.getNbLevel -> 
+nbL <= CLevel (nbLevel - 1).
+Proof.
+intros.
+unfold getNbLevel in *.
+destruct (gt_dec nbLevel 0).
+inversion H. 
+unfold CLevel.
+case_eq (lt_dec (nbLevel - 1) nbLevel); intros.
+simpl.
+omega.
+omega.
+assert (0 < nbLevel) by apply nbLevelNotZero.
+omega.
+Qed.
+
+Lemma getNbLevelEq : 
+forall nbL, 
+Some nbL = StateLib.getNbLevel -> 
+nbL = CLevel (nbLevel - 1).
+Proof.
+intros.
+unfold getNbLevel in *.
+destruct (gt_dec nbLevel 0).
+inversion H.
+destruct nbL.
+simpl in *.
+ 
+unfold CLevel.
+case_eq (lt_dec (nbLevel - 1) nbLevel); intros.
+inversion H.
+subst.
+f_equal.
+apply proof_irrelevance.
+assert (0 < nbLevel) by apply nbLevelNotZero.
+omega.
+now contradict H.
+Qed.
+
+
+(** beqPairs **)
 Lemma beqPairsTrue : 
 forall table1 idx1 table2 idx2 , table1 = table2 /\ idx1 = idx2 <->   
 beqPairs (table1, idx1) (table2, idx2) beqPage beqIndex = true.
@@ -373,103 +793,3 @@ destruct idx1, idx2. simpl in *. subst.
 assert (Hi = Hi0).
 apply proof_irrelevance. subst. trivial. *)
 Admitted.
-
-Lemma noteqIndex a b:
-a < tableSizeLowerBound -> b < tableSizeLowerBound -> a<>b ->  
-CIndex a <> CIndex b.
-Proof.
-intros. 
-apply indexEqFalse;
-assert (tableSize > tableSizeLowerBound).
-apply tableSizeBigEnough.
-unfold tableSizeLowerBound in *.
-omega.  apply tableSizeBigEnough.
-unfold tableSizeLowerBound in *.
-omega. apply tableSizeBigEnough. omega.
-Qed.
-
-Lemma CLevelMinusEq0 : 
-forall (a : level) b , CLevel (a -  b) = CLevel 0 ->   a = CLevel b \/ a < b. 
-Proof.
-intros.
-unfold CLevel in *.  
-case_eq (lt_dec (a - b) nbLevel );
-intros lab Hab; rewrite Hab in *.
-case_eq(lt_dec 0 nbLevel);
-intros l0 H0;
-rewrite H0 in*.
-inversion H.
-case_eq (lt_dec b nbLevel);
-intros lb Hb.
-simpl in *.
-apply NPeano.Nat.sub_0_le in H2.
-apply le_lt_or_eq in H2.
-destruct H2. 
-right; assumption.
-left.
-destruct a.
-simpl in *.
-subst.
-assert (Hl =  ADT.CLevel_obligation_1 b lb ) by 
-apply proof_irrelevance.
-subst. reflexivity.
-right; destruct a; simpl in *; omega.
-assert (0 < nbLevel) by apply nbLevelNotZero.
-now contradict H1.
-destruct a. simpl in *.
-omega.
-Qed.
-
-Lemma getNbLevelLe : 
-forall nbL, 
-Some nbL = StateLib.getNbLevel -> 
-nbL <= CLevel (nbLevel - 1).
-Proof.
-intros.
-unfold getNbLevel in *.
-destruct (gt_dec nbLevel 0).
-inversion H. 
-unfold CLevel.
-case_eq (lt_dec (nbLevel - 1) nbLevel); intros.
-simpl.
-omega.
-omega.
-assert (0 < nbLevel) by apply nbLevelNotZero.
-omega.
-Qed.
-
-Lemma getNbLevelEq : 
-forall nbL, 
-Some nbL = StateLib.getNbLevel -> 
-nbL = CLevel (nbLevel - 1).
-Proof.
-intros.
-unfold getNbLevel in *.
-destruct (gt_dec nbLevel 0).
-inversion H.
-destruct nbL.
-simpl in *.
- 
-unfold CLevel.
-case_eq (lt_dec (nbLevel - 1) nbLevel); intros.
-inversion H.
-subst.
-f_equal.
-apply proof_irrelevance.
-assert (0 < nbLevel) by apply nbLevelNotZero.
-omega.
-now contradict H.
-Qed.
-
-Lemma CIndexEq : 
-forall i : index, CIndex i = i. 
-Proof.
-intros.
-unfold CIndex.
-destruct i.
-simpl.
-case_eq(lt_dec i tableSize); intros.
-assert(ADT.CIndex_obligation_1 i l = Hi) by apply proof_irrelevance.
-subst. reflexivity.
-now contradict Hi.
-Qed.
